CCTests.lean
@@ -1,0 +1,12 @@
+import CCTests.Tests.RegAllocGoto
+import CCTests.Tests.LivermoreLoops
+import CCTests.Tests.OptEffectiveness
+import CCTests.Examples.ExecExamples
+import CCTests.Examples.WhileExamples
+import CCTests.Examples.TypedExamples
+import CCTests.Examples.CSEOptExamples
+import CCTests.Examples.ConstPropOptExamples
+import CCTests.Examples.DCEOptExamples
+import CCTests.Examples.LICMOptExamples
+import CCTests.Examples.ParserExamples
+import CCTests.Examples.PeepholeOptExamples
